graalir2/gendoc.sh
@@ -3,4 +3,4 @@
 isabelle build -d . -v -c semantics
 
 find output/document -type f -name "*.tex" -exec sed -n '/snip/,/endsnip/p' {} + | \
-    sed -e 's/isasymlongmapsto/isasymmapsto/g' > "../../papers/cpp-2021/snippets.tex"
+    sed -e 's/isasymhookrightarrow/isasymmapsto/g' > "../../papers/cpp-2021/snippets.tex"
